substitution

untypedLambda.v
@@ -1,13 +1,15 @@
 Require Import ssreflect.
+(*Require Import ssrnat.*)
 Require Import Arith.EqNat.
 Require Import Arith.Compare_dec.
+Require Import List.
 
 Definition var := nat.
 
 Inductive term :=
-  | Var : var -> term
-  | Lambda: term -> term
-  | App: term -> term -> term.
+| Var : var -> term
+| Lambda: term -> term
+| App: term -> term -> term.
 
 Check Lambda ( Lambda (Var 1)).
 
@@ -21,6 +23,45 @@ Fixpoint term_clos_aux (n : nat) (t: term): Prop :=
 Definition term_clos (t: term): Prop := term_clos_aux 1 t.
 
 Compute (term_clos (Lambda (Var 0))).
+
+Fixpoint C_aux (k: nat) (i: nat) (t: term): Prop :=
+  match t with
+    | Var v => lt v i
+    | App t1 t2 => (C_aux k i t1) /\ (C_aux k i t2)
+    | Lambda t1 => C_aux (k+1) i t1
+  end.
+
+Definition C (i: nat) (t: term): Prop := C_aux 0 i t.
+
+Lemma ind_Caux_pred: forall t: term, forall n k: nat,  C_aux k n t -> C_aux k (n+1) t. 
+Proof.
+  move => t n.
+  induction t.
+  move => k.
+  simpl.
+  move => h0.
+  Search _ "trans".
+  apply (Plus.lt_plus_trans v n 1).
+  done.
+  simpl.
+  move => k h0.
+  apply IHt.
+  done.
+  move => k.
+  simpl.
+  move => [h0 h1].
+  split.
+  apply IHt1.
+  done.
+  apply IHt2.
+  done.
+Qed.
+
+Lemma ind_C_pred: forall t: term, forall n: nat, C n t -> C (n+1) t.
+Proof.
+  move => t n.
+  apply (ind_Caux_pred t n 0).
+Qed.
 
 Fixpoint increase_k_fv (k: nat) (n:nat) (t:term): term :=
   match t with
@@ -43,3 +84,65 @@ Compute (term_clos (App (Lambda (Lambda (Var 2))) (Lambda ( Lambda (Var 0))))).
 Compute (increase_k_fv 0 0 (Lambda ( Lambda (Var 0)))).
 
 Compute (beta_eq (Lambda (Lambda (App (Var 1) (Lambda (App (Var 0) (Var 2)))))) (Lambda (App (Var 5) (Var 0)))).
+
+Fixpoint lifting (n: nat) (k: nat) (t: term): term :=
+  match t with
+    | Var i => if leb k i then Var (i+n) else Var i
+    | App t1 t2 => App (lifting n k t1) (lifting n k t2)
+    | Lambda t1 => Lambda (lifting n (k+1) t1)
+  end.
+
+Fixpoint substitution (i: nat) (t1: term) (t2: term): term :=
+  match t1 with
+    | Var k => if leb i k then (if beq_nat i k then lifting i 0 t2 else Var k) else Var (k-1)
+    | App t3 t4 => App (substitution i t3 t2) (substitution i t4 t2)
+    | Lambda t3 => Lambda (substitution (i+1) t3 t2)
+  end.
+
+(*Lemma substitution_invariance: forall t t1: term, (term_clos t) => substitution*)
+
+Fixpoint multiple_substitution (t: term) (lt: list term) (i: nat) (length: nat): term :=
+  match t with
+    | Var v => if (leb i v) && (leb v (i+length-1)) then substitution v (Var v) (nth (v - i) lt (Var v))  else Var v
+    | App t1 t2 => App (multiple_substitution t1 lt i length) (multiple_substitution t2 lt i length)
+    | Lambda t1 => Lambda (multiple_substitution t1 lt (i+1) length)
+  end.
+
+Lemma id_substitution: forall t: term, forall i: nat, multiple_substitution t nil i 0 = t.
+Proof.
+  move => t.
+  induction t.
+  move => i.
+  induction i.
+  simpl.
+  case v.
+  simpl.
+  done.
+  simpl.
+  done.
+  simpl.
+  case v.
+  simpl.
+  done.
+  move => n.
+  have:(((leb i n) && (leb (S n) (i + 0 - 0)))%bool = false).
+  Search "&&".  
+  apply Bool.andb_false_iff.
+  admit.
+  move => h0.
+  rewrite h0.
+  done.
+  simpl.
+  move => i.
+  rewrite IHt.
+  done.
+  simpl.
+  move => i.
+  rewrite IHt1.
+  rewrite IHt2.
+  done.
+Qed.
+
+Lemma no_index_sub: forall t u: term, forall i: nat, C i t -> substitution i t u = t.
+  Proof.
+    move => t u.
